

# Ground Stratified Induction for the Logic of Definitions

Nathan Guermond & Gopalan Nadathur

University of Minnesota Twin-Cities

December 12, 2025



# Outline

**Context:** The *logic of definitions* is

- A simply typed first order intuitionistic logic + definitions

# Outline

**Context:** The *logic of definitions* is

- A simply typed first order intuitionistic logic + definitions with
- a *stratification* condition to ensure consistency

# Outline

**Context:** The *logic of definitions* is

- A simply typed first order intuitionistic logic + definitions with
- a *stratification* condition to ensure consistency

**Previous work:**

- Tiu [2012] showed *ground stratification* is sufficient for consistency

# Outline

**Context:** The *logic of definitions* is

- A simply typed first order intuitionistic logic + definitions with
- a *stratification* condition to ensure consistency

**Previous work:**

- Tiu [2012] showed *ground stratification* is sufficient for consistency
- We showed [2025] that we can mix *ground stratified definitions* with *inductive definitions*

# Outline

**Context:** The *logic of definitions* is

- A simply typed first order intuitionistic logic + definitions with
- a *stratification* condition to ensure consistency

**Previous work:**

- Tiu [2012] showed *ground stratification* is sufficient for consistency
- We showed [2025] that we can mix *ground stratified definitions* with *inductive definitions*
- **Question:** Can we have ground stratified *inductive* definitions?

# Outline

**Context:** The *logic of definitions* is

- A simply typed first order intuitionistic logic + definitions with
- a *stratification* condition to ensure consistency

**Previous work:**

- Tiu [2012] showed *ground stratification* is sufficient for consistency
- We showed [2025] that we can mix *ground stratified definitions* with *inductive definitions*
- **Question:** Can we have ground stratified *inductive* definitions?

**This work:**

- We show that ground stratified inductive definitions are consistent with a new induction rule

# Outline

**Context:** The *logic of definitions* is

- A simply typed first order intuitionistic logic + definitions with
- a *stratification* condition to ensure consistency

**Previous work:**

- Tiu [2012] showed *ground stratification* is sufficient for consistency
- We showed [2025] that we can mix *ground stratified definitions* with *inductive definitions*
- **Question:** Can we have ground stratified *inductive* definitions?

**This work:**

- We show that ground stratified inductive definitions are consistent with a new induction rule
- This allows us to encode **inductive** logical relations defined by **recursion** on some argument



# Definitions

## Definition (Definition)

A *definition* for a predicate  $p$  is a set of clauses of the form

$$p\ t_1\ \dots\ t_n \stackrel{\Delta}{=} B$$

for terms  $t_1, \dots, t_n$  and a formula  $B$ .

# Definitions

## Definition (Definition)

A *definition* for a predicate  $p$  is a set of clauses of the form

$$p\ t_1\ \dots\ t_n \stackrel{\Delta}{=} B$$

for terms  $t_1, \dots, t_n$  and a formula  $B$ .

Eg. Given a signature for naturals:

$\mathbf{z} : tm$

$\mathbf{suc} : tm \rightarrow tm$

# Definitions

## Definition (Definition)

A *definition* for a predicate  $p$  is a set of clauses of the form

$$p \ t_1 \ \dots \ t_n \stackrel{\Delta}{=} B$$

for terms  $t_1, \dots, t_n$  and a formula  $B$ .

Eg. Given a signature for naturals:

$\mathbf{z} : tm$

$\mathbf{suc} : tm \rightarrow tm$

We define the predicates  $\mathbf{nat} : tm \rightarrow \mathbf{prop}$

$$\mathbf{nat} \ \mathbf{z} \stackrel{\Delta}{=} \top$$

$$\mathbf{nat} \ (\mathbf{suc} \ X) \stackrel{\Delta}{=} \mathbf{nat} \ X$$

# Definitions

## Definition (Definition)

A *definition* for a predicate  $p$  is a set of clauses of the form

$$p\ t_1\ \dots\ t_n \stackrel{\Delta}{=} B$$

for terms  $t_1, \dots, t_n$  and a formula  $B$ .

Eg. Given a signature for naturals:

$z : tm$

$suc : tm \rightarrow tm$

We define the predicates  $nat : tm \rightarrow \mathbf{prop}$  and  $even : tm \rightarrow \mathbf{prop}$

$$nat\ z \stackrel{\Delta}{=} \top$$

$$nat\ (suc\ X) \stackrel{\Delta}{=} nat\ X$$

$$even\ z \stackrel{\Delta}{=} \top$$

$$even\ (suc\ (suc\ X)) \stackrel{\Delta}{=} even\ X$$

# Unfolding definitions

The logic comes with *unfolding rules* for definitions.

# Unfolding definitions

The logic comes with *unfolding rules* for definitions.

Unfolding a goal formula corresponds to **pattern matching**:

$$\implies \text{even} (\text{suc} (\text{suc } z))$$

# Unfolding definitions

The logic comes with *unfolding rules* for definitions.

Unfolding a goal formula corresponds to **pattern matching**:

$$\implies \text{even} (\text{suc} (\text{suc } z))$$

Unfolding a hypothesis corresponds to **case analysis**:

$$\text{nat } x \implies (x = z) \vee \exists y. (x = \text{suc } y) \wedge (\text{nat } y)$$

# Unfolding definitions

The logic comes with *unfolding rules* for definitions.

Unfolding a goal formula corresponds to **pattern matching**:

$$\Longrightarrow \text{even} (\text{suc} (\text{suc } z))$$

Unfolding a hypothesis corresponds to **case analysis**:

$$\text{nat } x \Longrightarrow (x = z) \vee \exists y. (x = \text{suc } y) \wedge (\text{nat } y)$$

$$\text{even} (\text{suc } z) \Longrightarrow \perp$$



# Unfolding definitions

The logic comes with *unfolding rules* for definitions.

Unfolding a goal formula corresponds to **pattern matching**:

$$\Longrightarrow \text{even} (\text{suc} (\text{suc } z))$$

Unfolding a hypothesis corresponds to **case analysis**:

$$\text{nat } x \Longrightarrow (x = z) \vee \exists y. (x = \text{suc } y) \wedge (\text{nat } y)$$

$$\text{even} (\text{suc } z) \Longrightarrow \perp$$

We **cannot** prove

$$\text{nat } x \Longrightarrow (\text{even } x) \vee (\text{even} (\text{suc } x))$$

# Unfolding definitions

The logic comes with *unfolding rules* for definitions.

Unfolding a goal formula corresponds to **pattern matching**:

$$\Longrightarrow \text{even} (\text{suc} (\text{suc } z))$$

Unfolding a hypothesis corresponds to **case analysis**:

$$\text{nat } x \Longrightarrow (x = z) \vee \exists y. (x = \text{suc } y) \wedge (\text{nat } y)$$

$$\text{even} (\text{suc } z) \Longrightarrow \perp$$

We **cannot** prove

$$\boxed{\text{nat } x} \Longrightarrow (\text{even } x) \vee (\text{even} (\text{suc } x))$$

# Unfolding definitions

The logic comes with *unfolding rules* for definitions.

Unfolding a goal formula corresponds to **pattern matching**:

$$\Longrightarrow \text{even} (\text{succ} (\text{succ } z))$$

Unfolding a hypothesis corresponds to **case analysis**:

$$\text{nat } x \Longrightarrow (x = z) \vee \exists y. (x = \text{succ } y) \wedge (\text{nat } y)$$

$$\text{even} (\text{succ } z) \Longrightarrow \perp$$

We **cannot** prove

$$\left\{ \begin{array}{ll} \Longrightarrow & (\text{even } z) \vee (\text{even} (\text{succ } z)) \\ \text{nat } y & \Longrightarrow (\text{even} (\text{succ } y)) \vee (\text{even} (\text{succ} (\text{succ } y))) \end{array} \right.$$

# Unfolding definitions

The logic comes with *unfolding rules* for definitions.

Unfolding a goal formula corresponds to **pattern matching**:

$$\Longrightarrow \text{even} (\text{suc} (\text{suc } z))$$

Unfolding a hypothesis corresponds to **case analysis**:

$$\text{nat } x \Longrightarrow (x = z) \vee \exists y. (x = \text{suc } y) \wedge (\text{nat } y)$$

$$\text{even} (\text{suc } z) \Longrightarrow \perp$$

We **cannot** prove

$$\left\{ \begin{array}{ll} & \Longrightarrow (\text{even } z) \\ \text{nat } y & \Longrightarrow (\text{even} (\text{suc } y)) \vee (\text{even} (\text{suc} (\text{suc } y))) \end{array} \right.$$

# Unfolding definitions

The logic comes with *unfolding rules* for definitions.

Unfolding a goal formula corresponds to **pattern matching**:

$$\Longrightarrow \text{even} (\text{suc} (\text{suc } z))$$

Unfolding a hypothesis corresponds to **case analysis**:

$$\text{nat } x \Longrightarrow (x = z) \vee \exists y. (x = \text{suc } y) \wedge (\text{nat } y)$$

$$\text{even} (\text{suc } z) \Longrightarrow \perp$$

We **cannot** prove

$$\left\{ \begin{array}{ll} & \Longrightarrow \top \\ \text{nat } y & \Longrightarrow (\text{even} (\text{suc } y)) \vee (\text{even} (\text{suc} (\text{suc } y))) \end{array} \right.$$

# Unfolding definitions

The logic comes with *unfolding rules* for definitions.

Unfolding a goal formula corresponds to **pattern matching**:

$$\Longrightarrow \text{even} (\text{suc} (\text{suc } z))$$

Unfolding a hypothesis corresponds to **case analysis**:

$$\text{nat } x \Longrightarrow (x = z) \vee \exists y. (x = \text{suc } y) \wedge (\text{nat } y)$$

$$\text{even} (\text{suc } z) \Longrightarrow \perp$$

We **cannot** prove

$$\left\{ \begin{array}{ll} & \Longrightarrow \top \quad \checkmark \\ \text{nat } y & \Longrightarrow (\text{even} (\text{suc } y)) \vee (\text{even} (\text{suc} (\text{suc } y))) \end{array} \right.$$

# Unfolding definitions

The logic comes with *unfolding rules* for definitions.

Unfolding a goal formula corresponds to **pattern matching**:

$$\Longrightarrow \text{even} (\text{suc} (\text{suc } z))$$

Unfolding a hypothesis corresponds to **case analysis**:

$$\text{nat } x \Longrightarrow (x = z) \vee \exists y. (x = \text{suc } y) \wedge (\text{nat } y)$$

$$\text{even} (\text{suc } z) \Longrightarrow \perp$$

We **cannot** prove

$$\left\{ \begin{array}{ll} \Longrightarrow \top & \checkmark \\ \text{nat } y \Longrightarrow (\text{even} (\text{suc } y)) \vee (\text{even} (\text{suc} (\text{suc } y))) & \end{array} \right.$$

# Unfolding definitions

The logic comes with *unfolding rules* for definitions.

Unfolding a goal formula corresponds to **pattern matching**:

$$\Longrightarrow \text{even} (\text{suc} (\text{suc } z))$$

Unfolding a hypothesis corresponds to **case analysis**:

$$\text{nat } x \Longrightarrow (x = z) \vee \exists y. (x = \text{suc } y) \wedge (\text{nat } y)$$

$$\text{even} (\text{suc } z) \Longrightarrow \perp$$

We **cannot** prove

$$\left\{ \begin{array}{ll} & \Longrightarrow \top \quad \checkmark \\ \text{nat } y & \Longrightarrow (\text{even} (\text{suc } y)) \vee (\text{even } y) \end{array} \right.$$



# Unfolding definitions

The logic comes with *unfolding rules* for definitions.

Unfolding a goal formula corresponds to **pattern matching**:

$$\implies \text{even} (\text{suc} (\text{suc } z))$$

Unfolding a hypothesis corresponds to **case analysis**:

$$\text{nat } x \implies (x = z) \vee \exists y. (x = \text{suc } y) \wedge (\text{nat } y)$$

$$\text{even} (\text{suc } z) \implies \perp$$

We **cannot** prove

$$\left\{ \begin{array}{ll} & \implies \top \quad \checkmark \\ \text{nat } y & \implies (\text{even} (\text{suc } y)) \vee (\text{even } y) \quad \times \end{array} \right.$$

To do this, we need *nat* to be an *inductive definition*!

# Inductive definitions

A predicate  $S$  is an *inductive invariant* for  $nat$  if it satisfies

$$\implies S\ z$$

$$S\ x \implies S\ (\text{succ}\ x)$$

# Inductive definitions

A predicate  $S$  is an *inductive invariant* for  $nat$  if it satisfies

$$\implies S\ z$$

$$S\ x \implies S\ (\text{succ}\ x)$$

The *inductive rule* for  $nat$  allows us to conclude

$$nat\ x \implies S\ x$$

# Inductive definitions

A predicate  $S$  is an *inductive invariant* for  $nat$  if it satisfies

$$\implies S\ z$$

$$S\ x \implies S\ (\text{succ}\ x)$$

The *inductive rule* for  $nat$  allows us to conclude

$$nat\ x \implies S\ x$$

We can show the following is an invariant for  $nat$

$$S := \lambda x. (\text{even}\ x) \vee (\text{even}\ (\text{succ}\ x))$$

# Inductive definitions

A predicate  $S$  is an *inductive invariant* for  $nat$  if it satisfies

$$\implies S\ z$$

$$S\ x \implies S\ (\text{succ}\ x)$$

The *inductive rule* for  $nat$  allows us to conclude

$$nat\ x \implies (even\ x) \vee (even\ (\text{succ}\ x))$$

We can show the following is an invariant for  $nat$

$$S := \lambda x. (even\ x) \vee (even\ (\text{succ}\ x))$$

# Inductive definitions

An *inductive* definition for  $p$  is a set of clauses

$$p \vec{t}_1 \stackrel{\mu}{=} B_1 \qquad \dots \qquad p \vec{t}_n \stackrel{\mu}{=} B_n$$

# Inductive definitions

An *inductive* definition for  $p$  is a set of clauses

$$p \vec{t}_1 \stackrel{\mu}{=} B_1 \qquad \dots \qquad p \vec{t}_n \stackrel{\mu}{=} B_n$$

An *inductive invariant*  $S$  for  $p$  is a predicate satisfying

$$B_i[S/p] \implies S \vec{t}_i$$

for each clause  $p \vec{t}_i \stackrel{\mu}{=} B_i$ .

# Inductive definitions

An *inductive* definition for  $p$  is a set of clauses

$$p \vec{t}_1 \stackrel{\mu}{=} B_1 \qquad \dots \qquad p \vec{t}_n \stackrel{\mu}{=} B_n$$

An *inductive invariant*  $S$  for  $p$  is a predicate satisfying

$$B_i[S/p] \implies S \vec{t}_i$$

for each clause  $p \vec{t}_i \stackrel{\mu}{=} B_i$ .

The *induction rule* says that whenever

$$\Gamma, S \vec{t} \implies C$$

then

$$\Gamma, p \vec{t} \implies C$$



# Stratification

If we allow *any* definition, eg.

$$p \stackrel{\Delta}{=} p \supset \perp$$

we can prove  $\vdash \perp$ , which makes the logic **inconsistent**!

# Stratification

If we allow *any* definition, eg.

$$p \stackrel{\Delta}{=} p \supset \perp$$

we can prove  $\vdash \perp$ , which makes the logic **inconsistent**!

## Definition (Stratification)

A collection of definitions is *stratified* if predicates can be ordered such that those appearing to the left of an implication in the body  $B$  of a definition  $p \vec{t} \stackrel{\Delta}{=} B$  have already been defined.

# Stratification

If we allow *any* definition, eg.

$$p \triangleq p \supset \perp$$

we can prove  $\vdash \perp$ , which makes the logic **inconsistent**!

## Definition (Stratification)

A collection of definitions is *stratified* if predicates can be ordered such that those appearing to the left of an implication in the body  $B$  of a definition  $p \vec{t} \triangleq B$  have already been defined.

**Eg.** The following can be stratified:

$$q \triangleq q$$

$$p \triangleq q \supset \perp$$

# Ground stratification

Suppose we've defined a *reduction relation* on *simply-typed*  $\lambda$ -terms:

$$\text{step } T \ U$$

# Ground stratification

Suppose we've defined a *reduction relation* on *simply-typed*  $\lambda$ -terms:

$$\text{step } T \ U$$

We define *strong normalizability*:

$$\text{sn } T \stackrel{\mu}{=} \forall u. (\text{step } T \ u) \supset (\text{sn } u)$$

# Ground stratification

Suppose we've defined a *reduction relation* on *simply-typed*  $\lambda$ -terms:

$$\text{step } T \ U$$

We define *strong normalizability*:

$$\text{sn } T \stackrel{\mu}{=} \forall u. (\text{step } T \ u) \supset (\text{sn } u)$$

Now define *reducibility*:

$$\begin{aligned} \text{red unit } t &\stackrel{\Delta}{=} \text{sn } t \\ \text{red } (A \Rightarrow B) \ t &\stackrel{\Delta}{=} \forall u. (\text{red } A \ u) \supset (\text{red } B \ (\text{app } t \ u)) \end{aligned}$$

# Ground stratification

Suppose we've defined a *reduction relation* on *simply-typed*  $\lambda$ -terms:

$$\text{step } T \ U$$

We define *strong normalizability*:

$$\text{sn } T \stackrel{\mu}{=} \forall u. (\text{step } T \ u) \supset (\text{sn } u)$$

Now define *reducibility*:

$$\begin{aligned} \text{red unit } t &\stackrel{\Delta}{=} \text{sn } t \\ \text{red } (A \Rightarrow B) \ t &\stackrel{\Delta}{=} \forall u. (\text{red } A \ u) \supset (\text{red } B \ (\text{app } t \ u)) \end{aligned}$$

**Remark:** *red* is *not* stratified

# Ground stratification

Suppose we've defined a *reduction relation* on *simply-typed*  $\lambda$ -terms:

$$\text{step } T \ U$$

We define *strong normalizability*:

$$\text{sn } T \stackrel{\mu}{=} \forall u. (\text{step } T \ u) \supset (\text{sn } u)$$

Now define *reducibility*:

$$\begin{aligned} \text{red unit } t &\stackrel{\Delta}{=} \text{sn } t \\ \text{red } (A \Rightarrow B) \ t &\stackrel{\Delta}{=} \forall u. (\text{red } A \ u) \supset (\text{red } B \ (\text{app } t \ u)) \end{aligned}$$

**Remark:** *red* is *not* stratified; it is defined by *recursion* on the type argument. Tiu [2012] called this **ground stratification** and showed that such definitions are consistent.



# Can inductive definitions be ground stratified?

What if we want *red* to be inductive?

$$\begin{aligned} \text{red unit } t &\triangleq \text{sn } t \\ \text{red } (A \Rightarrow B) t &\triangleq \forall u. (\text{red } A u) \supset (\text{red } B (\text{app } t u)) \end{aligned}$$

# Can inductive definitions be ground stratified?

What if we want *red* to be inductive?

$$\begin{aligned}
 \text{red unit } t & \stackrel{\mu}{=} \text{sn } t \\
 \text{red } (A \Rightarrow B) & \stackrel{\mu}{=} \forall u. (\text{red } A \ u) \supset (\text{red } B \ (\text{app } t \ u))
 \end{aligned}$$

# Can inductive definitions be ground stratified?

What if we want *red* to be inductive?

$$\begin{aligned}
 \text{red unit } t &\stackrel{\mu}{=} \text{sn } t \\
 \text{red } (A \Rightarrow B) &\stackrel{\mu}{=} \forall u. (\text{red } A \ u) \supset (\text{red } B \ (\text{app } t \ u))
 \end{aligned}$$

With the current induction rule, ground stratified inductive definitions may lead to inconsistencies [GN 2025]<sup>1</sup>!

<sup>1</sup>Ground stratification for a logic of definitions with induction

# Can inductive definitions be ground stratified?

What if we want *red* to be inductive?

$$\begin{aligned}
 \text{red unit } t &\stackrel{\mu}{=} \text{sn } t \\
 \text{red } (A \Rightarrow B) &\stackrel{\mu}{=} \forall u. (\text{red } A \ u) \supset (\text{red } B \ (\text{app } t \ u))
 \end{aligned}$$

With the current induction rule, ground stratified inductive definitions may lead to inconsistencies [GN 2025]<sup>1</sup>!

**We must therefore modify the induction rule!**

<sup>1</sup>Ground stratification for a logic of definitions with induction

# Ground stratified inductive definitions

An *inductive invariant*  $S$  for  $p$  is a predicate such that for each clause,

$$B_i[S/p] \implies S \vec{t}_i$$

# Ground stratified inductive definitions

## New definition:

An *inductive invariant*  $S$  for  $p$  is a predicate such that for each clause,

$$B_i^+ S \implies S \vec{t}_i$$

where  $B^+$  is obtained from a formula  $B$  by abstracting all *strictly positive* occurrences of  $p$ , eg.

$$((p \vec{t}_1 \supset p \vec{t}_2) \supset p \vec{t}_3)^+ := \lambda S. ((p \vec{t}_1 \supset p \vec{t}_2) \supset S \vec{t}_3)$$

# Ground stratified inductive definitions

## New definition:

An *inductive invariant*  $S$  for  $p$  is a predicate such that for each clause,

$$B_i^+ S \implies S \vec{t}_i$$

where  $B^+$  is obtained from a formula  $B$  by abstracting all *strictly positive* occurrences of  $p$ , eg.

$$((p \vec{t}_1 \supset p \vec{t}_2) \supset p \vec{t}_3)^+ := \lambda S. ((p \vec{t}_1 \supset p \vec{t}_2) \supset S \vec{t}_3)$$

If  $p$  is stratified, then  $B[S/p] = B^+ S$ , so this subsumes previous notion of inductive invariant.

# Consistency

## Theorem (Consistency)

*The logic of definitions with ground stratified definitions and ground stratified inductive definitions (with the new induction rule) is consistent.*



# Consistency

## Theorem (Consistency)

*The logic of definitions with ground stratified definitions and ground stratified inductive definitions (with the new induction rule) is consistent.*

The key lemma needed is:

## Lemma (Unfolding lemma)

*For any formula  $C$ , inductive definition  $p$ , and inductive invariant  $S$ , the following holds*

$$C \implies C^+ S.$$

# Example Application

**Application:** Strong normalization for *System T*:

Simply typed  $\lambda$ -calculus + natural number recursion

# Example Application

**Application:** Strong normalization for *System T*:

Simply typed  $\lambda$ -calculus + natural number recursion

We adapt Martin-Löf's [1971] *computability predicate* to System T:

$$\text{red nat } z \stackrel{\mu}{=} \top$$

$$\text{red nat } (\text{succ } X) \stackrel{\mu}{=} \text{red nat } X$$

$$\text{red } (A \Rightarrow B) (\text{lam } S) \stackrel{\mu}{=} \forall u. (\text{red } A \ u) \supset (\text{red } B \ (S \ u))$$

$$\text{red } B \ T \stackrel{\mu}{=} (\text{neutral } T) \wedge \forall u. (\text{step } T \ u) \supset \text{red } B \ u$$

# Example Application

**Application:** Strong normalization for *System T*:

Simply typed  $\lambda$ -calculus + natural number recursion

We adapt Martin-Löf's [1971] *computability predicate* to System T:

$$\text{red nat } z \stackrel{\mu}{=} \top$$

$$\text{red nat } (\text{succ } X) \stackrel{\mu}{=} \text{red nat } X$$

$$\text{red } (A \Rightarrow B) (\text{lam } S) \stackrel{\mu}{=} \forall u. (\text{red } A \ u) \supset (\text{red } B \ (S \ u))$$

$$\text{red } B \ T \stackrel{\mu}{=} (\text{neutral } T) \wedge \forall u. (\text{step } T \ u) \supset \text{red } B \ u$$

Strong normalization requires induction on reducibility

# Conclusion, related, and future work

**Conclusion:** The logic of definitions with ground stratified definitions is compatible with ground stratified inductive definitions.

## Conclusion, related, and future work

**Conclusion:** The logic of definitions with ground stratified definitions is compatible with ground stratified inductive definitions.

**Future directions:**

1. Show that ground stratified induction is compatible with other features of the *Abella* proof assistant

# Conclusion, related, and future work

**Conclusion:** The logic of definitions with ground stratified definitions is compatible with ground stratified inductive definitions.

**Future directions:**

1. Show that ground stratified induction is compatible with other features of the *Abella* proof assistant
2. Relate ground stratified inductive definitions in the logic of definitions with *inductive-recursive* definitions in type theory

# Conclusion, related, and future work

**Conclusion:** The logic of definitions with ground stratified definitions is compatible with ground stratified inductive definitions.

## Future directions:

1. Show that ground stratified induction is compatible with other features of the *Abella* proof assistant
2. Relate ground stratified inductive definitions in the logic of definitions with *inductive-recursive* definitions in type theory
3. Generalize the induction rule to work with all (non-strictly) *positive* inductive invariants (ie.  $B^+$  should abstract all positive occurrences of  $p$ )



# Conclusion, related, and future work

**Conclusion:** The logic of definitions with ground stratified definitions is compatible with ground stratified inductive definitions.

## Future directions:

1. Show that ground stratified induction is compatible with other features of the *Abella* proof assistant
2. Relate ground stratified inductive definitions in the logic of definitions with *inductive-recursive* definitions in type theory
3. Generalize the induction rule to work with all (non-strictly) *positive* inductive invariants (ie.  $B^+$  should abstract all positive occurrences of  $p$ )

**Thank you!**